formulation to suit labeled traces

theories/Traces.v
@@ -8,16 +8,16 @@ Ltac invs h := inversion h; subst => {h}.
 
 Section Traces.
 
-Context {A : Type}.
+Context {A B : Type}.
 
 CoInductive trace : Type  :=
 | Tnil : A -> trace
-| Tcons : A -> trace -> trace.
+| Tcons : A -> B -> trace -> trace.
 
 Definition trace_decompose (tr: trace): trace :=
 match tr with
-| Tnil st => Tnil st
-| Tcons a tr' => Tcons a tr'
+| Tnil a => Tnil a
+| Tcons a b tr' => Tcons a b tr'
 end.
 
 Lemma trace_destr:
@@ -25,82 +25,77 @@ forall tr, tr = trace_decompose tr.
 Proof. case => //=. Qed.
 
 CoInductive bisim: trace -> trace -> Prop :=
-| bisim_nil: forall st,
-  bisim (Tnil st) (Tnil st)
-| bisim_cons: forall e tr tr',
+| bisim_nil: forall a,
+  bisim (Tnil a) (Tnil a)
+| bisim_cons: forall a b tr tr',
   bisim tr tr' ->
-  bisim (Tcons e tr) (Tcons e tr').
+  bisim (Tcons a b tr) (Tcons a b tr').
 
 Lemma bisim_refl : forall tr, bisim tr tr. 
-Proof. 
-cofix CIH. case.
-- move => st. by apply bisim_nil. 
-- move => st tr.
-  apply bisim_cons.
-  exact: CIH.
+Proof.
+cofix CIH.
+case => [a|a b tr]; first exact: bisim_nil.
+apply bisim_cons.
+exact: CIH.
 Qed.
 
 Lemma bisim_sym : forall tr1 tr2, bisim tr1 tr2 -> bisim tr2 tr1. 
 Proof.
-cofix CIH. case. 
-- move => s tr2 h1. invs h1.  by apply: bisim_nil.  
-- move => s tr0 tr1 h1. invs h1.
-  apply: bisim_cons.
-  exact: (CIH _ _ H2).
+cofix CIH.
+case => [a|a b tr1] tr2 Hbs; invs Hbs; first exact: bisim_nil.
+by apply: bisim_cons; apply (CIH _ _ H3).
 Qed.
 
 Lemma bisim_trans : forall tr1 tr2 tr3,
 bisim tr1 tr2 -> bisim tr2 tr3 -> bisim tr1 tr3. 
 Proof.
-cofix CIH. case.  
-- move => st tr0 tr1 h1 h2. invs h1. invs h2. by apply: bisim_nil.
-- move => st tr0 tr1 tr2 h1 h2. invs h1. invs h2.
-  apply: bisim_cons.
-  exact: (CIH _ _ _ H2 H3).
+cofix CIH. 
+case => [a|a b tr1] tr2 tr0 Hbs Hbs'; invs Hbs; invs Hbs'; first exact: bisim_nil.
+apply: bisim_cons.
+exact: CIH _ _ _ H3 H4.
 Qed.
 
 CoFixpoint trace_append (tr tr': trace): trace :=
 match tr with
-| Tnil st => tr'
-| Tcons e tr0 => Tcons e (trace_append tr0 tr')
+| Tnil a => tr'
+| Tcons a b tr0 => Tcons a b (trace_append tr0 tr')
 end.
 
 Infix "+++" := trace_append (at level 60, right associativity).
 
-Lemma trace_append_nil: forall st tr, (Tnil st) +++ tr = tr.
+Lemma trace_append_nil: forall a tr, (Tnil a) +++ tr = tr.
 Proof. 
-move => st tr.
-rewrite [Tnil st +++ tr]trace_destr.
+move => a tr.
+rewrite [Tnil a +++ tr]trace_destr.
 by case tr.
 Qed.
 
-Lemma trace_append_cons: forall e tr tr',
- (Tcons e tr) +++ tr' = Tcons e (tr +++ tr').
+Lemma trace_append_cons: forall a b tr tr',
+ (Tcons a b tr) +++ tr' = Tcons a b (tr +++ tr').
 Proof.
-move => st tr tr'.
-rewrite [Tcons st tr +++ tr']trace_destr.
+move => a b tr tr'.
+rewrite [Tcons a b tr +++ tr']trace_destr.
 by case tr.
 Qed.
 
 Lemma trace_eq_append: forall tr1 tr2 tr3 tr4, 
  bisim tr1 tr2 -> bisim tr3 tr4 -> bisim (tr1 +++ tr3) (tr2 +++ tr4).
 Proof. 
-cofix CIH. case. 
-- move => st1 tr1 tr2 tr3 h1 h2. invs h1.
-  do 2 rewrite trace_append_nil.
-  exact: h2.
-- move => st tr1 tr2 tr3 tr4 h1 h2. invs h1. 
-  do 2 rewrite trace_append_cons.
+cofix CIH. 
+case => [a|a b tr1] tr2 tr3 tr4 Hbs1 Hbs2; invs Hbs1.
+- do 2 rewrite trace_append_nil.
+  exact: Hbs2.
+- do 2 rewrite trace_append_cons.
   apply: bisim_cons.
-  exact: (CIH _ _ _ _ H2 h2).
+  exact: CIH.
 Qed.
 
 Definition hd tr :=
-match tr with Tnil st => st | Tcons st tr0 => st end.
+match tr with Tnil st => st | Tcons a b tr0 => a end.
 
 Lemma bisim_hd: forall tr0 tr1, bisim tr0 tr1 -> hd tr0 = hd tr1. 
-Proof. 
-move => tr0 tr1 h0. by invs h0.
+Proof.
+by move => tr0 tr1 h0; invs h0.
 Qed.
 
 End Traces.
